When inlining the body of a predicate (in a proof obligation--via TrSplitExpr), use the instantiated types of the predicate's type parameters.  This delays the introduction of some boxes in the translation, which for some useful examples gives rise to better proving.

Source/Dafny/DafnyAst.cs
@@ -3907,7 +3907,7 @@ namespace Microsoft.Dafny {
     public readonly Expression/*!*/ Receiver;
     public readonly IToken OpenParen;  // can be null if Args.Count == 0
     public readonly List<Expression/*!*/>/*!*/ Args;
-    public Dictionary<TypeParameter, Type> TypeArgumentSubstitutions;  // created, initialized, and used by resolution (could be deleted once all of resolution is done)
+    public Dictionary<TypeParameter, Type> TypeArgumentSubstitutions;  // created, initialized, and used by resolution (and also used by translation)
     public enum CoCallResolution { No, Yes, NoBecauseFunctionHasSideEffects, NoBecauseRecursiveCallsAreNotAllowedInThisContext, NoBecauseIsNotGuarded }
     public CoCallResolution CoCall = CoCallResolution.No;  // indicates whether or not the call is a co-recursive call; filled in by resolution
 
